Sequent.thy
@@ -9,16 +9,40 @@ text \<open>
 \label{sec:terms} The datatypes of terms and formulae are defined as follows:
 \<close>
 
-datatype ('a, 'b, 'c) form = 
-    Eq 'a 'a
-  | Concat 'a 'a 'a
-  | Extract 'a nat 'b 'a
-  | Replace 'a 'b 'c 'a
-  | ReplaceAll 'a 'b 'c 'a
-  | Member 'a \<open>('a) rexp\<close>
-  | Dis \<open>('a, 'b, 'c) form\<close> \<open>('a, 'b, 'c) form\<close>
-  | Con \<open>('a, 'b, 'c) form\<close> \<open>('a, 'b, 'c) form\<close>
-  | Neg \<open>('a, 'b, 'c) form\<close>
+type_synonym vname = \<open>char list\<close>
+type_synonym rep = string
+type_synonym crexp = "char rexp"
 
+
+datatype bterm = Var vname | Func \<open>bterm list\<close>
+
+datatype form = 
+    Eq vname bterm                      ("_ =:= _" [61,61] 61)
+  | Neq vname bterm                     ("_ =!= _" [61,61] 61)
+  | Concat vname vname vname            ("_ =:= _;;/ _" [61,61,61] 61)
+  | Member vname crexp
+  | NMember vname crexp
+  | Dis form form                      
+  | Con form form                      
+  | Neg form                           
+
+primrec eval :: "form \<Rightarrow> bool" where
+  "eval (Eq x y) = (x = y)" |
+  "eval (Concat z x y) = (z = x @ y)" |
+  "eval (Neg f) = (eval f)" |
+  "eval (Dis f1 f2) = (eval f1 \<or> eval f2)" |
+  "eval (Con f1 f2) = (eval f1 \<and> eval f2)" |
+  "eval (Member x e) = (x \<in> lang e)" |
+  "eval (Neq x y) = (x \<noteq> y)" |
+  "eval (NMember x e) = (x \<notin> lang e)"
+
+inductive SC :: \<open>form list \<Rightarrow> bool\<close> (\<open>\<turnstile> _\<close> 0) where
+  AlphaNegNeg: \<open>\<turnstile> A # G \<Longrightarrow> \<turnstile> Neg (Neg A) # G\<close>
+| AlphaNegOr: \<open>\<turnstile> Neg A # Neg B # G \<Longrightarrow> \<turnstile> Neg (Dis A B) # G\<close>
+| AlphaCon: \<open>\<turnstile> A # B # G \<Longrightarrow> \<turnstile> Con A B # G\<close>
+| BetaOr: \<open>\<turnstile> A # G \<Longrightarrow> \<turnstile> B # G \<Longrightarrow> \<turnstile> Or A B # G\<close>
+| BetaNegOr: \<open>\<turnstile> Neg A # G \<Longrightarrow> \<turnstile> Neg B # G \<Longrightarrow> \<turnstile> Neg (Con A B) # G\<close>
+| NotMember: \<open>lang e1 = UNIV - lang e2 \<Longrightarrow> \<turnstile> Member x e1 # G\<Longrightarrow> \<turnstile> NMember x e2  # G\<close>
+| NEq : \<open>\<turnstile> Neq x y # (Func y flist) # G \<Longrightarrow> Neq x )\<close>
 
 end
